snap. figuring out universe problems

experiments/DeeperShallowEmbedding.fst
@@ -5,27 +5,22 @@ open FStar.Universe
 
 #set-options "--print_universes"
 
-val ctx : Type u#(4+1)
-let ctx = Type u#4
+(** Shallow Embedding of DTT in F* - Figure 2 *)
 
-val typ : ctx -> Type u#(4+1)
-let typ cs = cs -> Type u#4
+val ctx : Type u#(a+1)
+let ctx = Type u#a
 
-(**
-let typ0 = fun (cs:ctx) -> cs -> Type u#0
-let typ1 = fun (cs:ctx) -> cs -> Type u#1
-let typ2 = fun (cs:ctx) -> cs -> Type u#2
-let typ3 = fun (cs:ctx) -> cs -> Type u#3
-**)
+val typ : ctx u#a -> Type u#(a+1)
+let typ cs = cs -> Type u#a
 
 val empty_ctx : ctx
 let empty_ctx : ctx = raise_t unit // or true?
 
-val cons : cs:ctx -> typ cs -> ctx
+val cons : cs:ctx u#a -> typ u#a cs -> ctx u#a
 let cons cs t = 
   c:cs & t c
 
-val var : cs:ctx  -> typ cs -> Type u#4
+val var : cs:ctx u#a -> typ u#a cs -> Type u#a
 let var cs t = (c:cs) -> t c
 
 val weakenT : #cs:ctx -> #t:(typ cs) -> typ cs -> typ (cons cs t)
@@ -40,10 +35,7 @@ let next x = fun (| c, _ |) -> x c
 val dt : #cs:ctx -> at:(typ cs) -> bt:(typ (cons cs at)) -> typ cs
 let dt #cs at bt = fun (c:cs) -> ((a : at c) -> bt (| c, a |))
 
-val u : #cs:ctx -> typ cs
-let u c = Type
-
-val term : cs:ctx -> typ cs -> Type u#4
+val term : cs:ctx u#a -> typ u#a cs -> Type u#a
 let term cs t = (c:cs) -> t c
 
 val lookup : #cs:ctx -> #t:(typ cs) -> icx:(var cs t) -> term cs t
@@ -54,3 +46,50 @@ let lambda e = fun c a -> e (| c, a |)
 
 val app : #cs:ctx -> #at:(typ cs) -> #bt:(typ (cons cs at)) -> term cs (dt at bt) -> (a : term cs at) -> term cs (fun c -> bt (| c, a c |))
 let app e1 e2 = fun c -> (e1 c) (e2 c)
+
+
+(** Deeper shallow embedding - Figure 3 **)
+noeq
+type dctx : (cs:ctx u#a) -> Type u#(a+1) =
+| Empty : dctx empty_ctx
+| Extend : (#cs:ctx) -> dctx cs -> t:(typ cs) -> dctx (cons cs t)
+
+noeq
+type dvar : #cs:ctx u#a -> dcs:(dctx cs) -> t:(typ cs) -> var cs t -> Type u#(a+1) =
+| Same : #cs:ctx -> #t:typ cs -> #dcs:dctx cs -> dvar (Extend dcs t) (weakenT t) same
+| Next : #cs:ctx -> #dcs:dctx cs -> #t:typ cs -> #at:_ -> #s:_ -> dvar #cs dcs at s -> dvar (Extend dcs t) (weakenT at) (next s)
+
+
+let typ0 (cs:ctx u#4) : Type u#4 = cs -> Type u#0
+let typ1 (cs:ctx u#4) : Type u#4 = cs -> Type u#1
+let typ2 (cs:ctx u#4) : Type u#4 = cs -> Type u#2
+let typ3 (cs:ctx u#4) : Type u#4 = cs -> Type u#3
+
+val u0 : #cs:ctx u#4 -> typ1 cs
+let u0 c = Type u#0
+
+val u1 : #cs:ctx u#4 -> typ2 cs
+let u1 c = Type u#1
+
+let lift0 (#cs:ctx u#4) (x:typ0 cs) : typ cs = fun c -> raise_t (x c)
+let lift1 (#cs:ctx u#4) (x:typ1 cs) : typ cs = fun c -> raise_t u#1 u#4 (x c)
+let lift2 (#cs:ctx u#4) (x:typ2 cs) : typ cs = fun c -> raise_t u#2 u#4 (x c)
+let lift3 (#cs:ctx u#4) (x:typ3 cs) : typ cs = fun c -> raise_t u#3 u#4 (x c)
+
+let vlift0 (#cs:ctx u#4) (x:typ0 cs) : term cs (lift1 u0) = fun c -> raise_val (x c)
+let vlift1 (#cs:ctx u#4) (x:typ1 cs) : term cs (lift2 u1) = fun c -> raise_val (x c)
+  
+val dt0 : #cs:ctx u#4 -> at:(typ0 cs) -> bt:(typ0 (cons cs (lift0 at))) -> typ0 cs
+let dt0 #cs at bt = fun (c:cs) -> ((a : at c) -> bt (| c, raise_val a |))
+
+val dt1 : #cs:ctx u#4 -> at:(typ1 cs) -> bt:(typ1 (cons cs (lift1 at))) -> typ1 cs
+let dt1 #cs at bt = fun (c:cs) -> ((a : at c) -> bt (| c, raise_val a |))
+
+noeq
+type dterm : #cs:ctx u#4 -> dcs:dctx cs -> t:typ cs -> term cs t -> Type u#5 =
+| Lambda : #cs:ctx -> #dcs:dctx cs -> #at:typ cs -> #bt:typ (cons cs at) -> #s:_ -> dterm (Extend dcs at) bt s -> dterm dcs (dt at bt) (lambda s)
+| Var : #cs:ctx -> #dcs:dctx cs -> #t:typ cs -> #s:term cs t -> dvar dcs t s -> dterm #cs dcs t s
+| App : #cs:ctx -> #dcs:dctx cs -> #at:typ cs -> #bt:typ (cons cs at) -> #s1:_ -> #s2:_ -> dterm dcs (dt at bt) s1 -> x:(dterm dcs at s2) -> dterm dcs (fun c -> bt (| c, s2 c |)) (app s1 s2)
+| Dt0 : #cs:ctx -> #dcs:dctx cs -> #at:typ0 cs -> #bt:_ -> dterm dcs (lift1 u0) (vlift0 at) -> dterm (Extend dcs (lift0 at)) (lift1 u0) (vlift0 bt) -> dterm dcs (lift1 u0) (vlift0 (dt0 at bt))
+| Dt1 : #cs:ctx -> #dcs:dctx cs -> #at:typ1 cs -> #bt:_ -> dterm dcs (lift2 u1) (vlift1 at) -> dterm (Extend dcs (lift1 at)) (lift2 u1) (vlift1 bt) -> dterm dcs (lift2 u1) (vlift1 (dt1 at bt))
+| U0 : #cs:ctx -> #dcs:dctx cs -> dterm dcs (lift2 u1) (vlift1 u0)
